CPL_Syntax.thy
@@ -6,10 +6,8 @@ begin
 
 (* ======================== Type Definitions ======================== *)
 
-type_synonym 'a Enumerable =  "'a::enum" \<comment>
- \<open>Note: It is possible to define types that must implement a class using this syntax\<close>
-type_synonym Variable =  "char Enumerable" \<comment>
- \<open>Note: Explain the caveats of using string. We will have to keep using char for now\<close>
+type_synonym 'a Enumerable =  "'a::enum" \<comment> \<open> Note: It is possible to define types that must implement a class using this syntax \<close>
+type_synonym Variable =  "char Enumerable" \<comment> \<open> Note: Explain the caveats of using string. We will have to keep using char for now \<close>
 type_synonym Relation =  "char Enumerable"
 datatype Formula =
 Atom (atom_rel: "Relation") (atom_vars: "Variable list") |
